MSFOL formalisation
 * added syntax, axioms, converting statements to AML patterns
 * added MSFOL proof rules
 * require to formalise MSFOL signature and structure

AML_definition.v
@@ -120,7 +120,7 @@ Definition simple := var ("x").
 Definition more := set ("A") _|_ ¬ (set "A").
 Definition complex :=
   var("A") ~> (var("B") ~> ¬(set("C"))) $
-  ex (evar_c("x")) , const("D") $ Bot _&_ Top.
+  ex (evar_c("x")) , set ("D") $ Bot _&_ Top.
 Definition custom_constructor := const ("ctor") $ var ("a").
 Definition predicate := const ("p") $ var ("x1") $ var ("x2").
 Definition function :=
@@ -165,18 +165,17 @@ match x, y with
 | evar_c id_x, evar_c id_y => String.eqb id_x id_y
 end.
 
+Definition set_singleton := fun x => set_add evar_eq_dec x List.nil.
+
 Fixpoint free_vars (phi : Sigma_pattern) : (ListSet.set EVar) :=
 match phi with
-| sp_var x => set_add evar_eq_dec x List.nil
+| sp_var x => set_singleton x
 | sp_set X => List.nil
 | sp_const sigma => List.nil
 | sp_app phi1 phi2 => set_union evar_eq_dec (free_vars phi1) (free_vars phi2)
 | sp_bottom => List.nil
 | sp_impl phi1 phi2 => set_union evar_eq_dec (free_vars phi1) (free_vars phi2)
-| sp_exists y phi =>
-    set_diff evar_eq_dec
-      (free_vars phi)
-      (set_add evar_eq_dec y List.nil)
+| sp_exists y phi => set_diff evar_eq_dec (free_vars phi) (set_singleton y )
 | sp_mu X phi => free_vars phi
 end.
 
@@ -358,15 +357,19 @@ Notation "phi1 !=~ phi2" := (NonEquality phi1 phi2) (at level 100).
 
 (* Membership *)
 Definition c_membership := (const ("membership")).
-Definition Membership (x : EVar) (phi : Sigma_pattern) :=
+Definition VarMembership (x : EVar) (phi : Sigma_pattern) :=
   ((c_membership $ (sp_var x)) $ phi).
-Notation "x -< phi" := (Membership x phi) (at level 30).
+Definition ConstMembership (x : Sigma) (phi : Sigma_pattern) :=
+  ((c_membership $ (sp_const x)) $ phi).
 
 (* Non-membership *)
 Definition c_non_membership := (const ("non-membership")).
-Definition NonMembership (x : EVar) (phi : Sigma_pattern) :=
+Definition VarNonMembership (x : EVar) (phi : Sigma_pattern) :=
   ((c_non_membership $ (sp_var x)) $ phi).
-Notation "x !-< phi" := (NonMembership x phi) (at level 30).
+Notation "x =< phi" := (VarMembership x phi) (at level 30).
+Definition ConstNonMembership (x : Sigma) (phi : Sigma_pattern) :=
+  ((c_non_membership $ (sp_const x)) $ phi).
+Notation "x -< phi" := (ConstMembership x phi) (at level 30).
 
 (* Set inclusion *)
 Definition c_set_incl := (const ("set inclusion")).
@@ -390,9 +393,13 @@ Inductive DefinednessOneStepEquivalence : Sigma_pattern -> Sigma_pattern -> Prop
     ((c_equality $ l) $ r) |->
     (Totality (sp_iff l r))
 
-| DOSE_membership {x : EVar} {phi : Sigma_pattern} :
+| DOSE_var_membership {x : EVar} {phi : Sigma_pattern} :
     ((c_membership $ (sp_var x)) $ phi) |->
     (Totality ((sp_var x) _&_ phi))
+
+| DOSE_const_membership {x : Sigma} {phi : Sigma_pattern} :
+    ((c_membership $ (sp_const x)) $ phi) |->
+    (Totality ((sp_const x) _&_ phi))
 
 | DOSE_set_inclusion {l r : Sigma_pattern} :
     ((c_set_incl $ l) $ r) |->
@@ -402,9 +409,13 @@ Inductive DefinednessOneStepEquivalence : Sigma_pattern -> Sigma_pattern -> Prop
     ((c_equality $ l) $ r) |->
     (¬ (Equality l r))
 
-| DOSE_non_membership {x : EVar} {phi : Sigma_pattern} :
+| DOSE_var_non_membership {x : EVar} {phi : Sigma_pattern} :
     ((c_non_membership $ (sp_var x)) $ phi) |->
-    (¬ (Membership x phi))
+    (¬ (VarMembership x phi))
+
+| DOSE_non_membership {x : Sigma} {phi : Sigma_pattern} :
+    ((c_non_membership $ (sp_const x)) $ phi) |->
+    (¬ (ConstMembership x phi))
 
 | DOSE_set_exclusion {l r : Sigma_pattern} :
     ((c_set_excl $ l) $ r) |->
@@ -722,6 +733,7 @@ Inductive Provable : Ensemble Sigma_pattern -> Sigma_pattern -> Prop :=
     theory |- (phi1 ~=~ phi2) -> theory |- (phi2 ~=~ phi1)
 
 | E_evar_subst
+  (* TODO: psi can be any pattern, not only Application_context *)
   (x : EVar) (phi1 phi2 psi : Sigma_pattern) (theory : Ensemble Sigma_pattern) :
     theory |- (phi1 ~=~ phi2) ->
     theory |- ((e_subst_var psi phi1 x) ~=~ (e_subst_var psi phi2 x))
@@ -754,7 +766,7 @@ Proof.
   eapply E_mod_pon.
   - eapply E_mod_pon.
     * eapply (hypothesis (¬(¬A)) theory).
-        (* TODO: write a tactic for this      *)
+        (* TODO: write a tactic for this *)
       + unfold theory. unfold In in *. unfold Add.
         eapply Union_introl. eapply Union_intror. reflexivity.
     * eapply (ext ((¬(¬A)) ~> (¬A ~> ¬(¬A))) theory).
@@ -784,6 +796,10 @@ Qed.
 Theorem Soundness :
   forall phi : Sigma_pattern, forall theory : Ensemble Sigma_pattern,
   (theory |- phi) -> (theory |= phi).
+(* Proof.
+  intros.
+              TODO
+  induction (proof_length (theory |= phi)). *)
 Admitted.
 
 Theorem Completeness :
@@ -794,74 +810,267 @@ Abort.
 (* ****************************New paper version**************************** *)
 
 (* Definition 9. MSFOL definition *)
-(* MSFOL_Signature :=
+(* record MSFOL_Signature := {
+  SortSet : Type
+  Functions : SortSet* -> SortSet
+  Predicates : SortSet*
+}. *)
 
-Inductive MSFOL_term : Set :=
-| MT_var ()
-| MT_fun
-.
-
-Inductive MSFOL_pattern : Set :=
-| MP_pred
-| MP_bottom
-| MP_app (l r : MSFOL_pattern)
-| MP_exists (x : MT_var) (phi : MSFOL_pattern)
-.
- *)
-(* Section 4.2 *)
-
-(* further axioms need to be appended to this axiom set *)
-Definition Gamma_MSFOL := Empty_set Sigma_pattern.
-
-Definition MSAFOL_Sort := const ("Sort").
-
-Definition Axiom_Sort (s : EVar) := s -< MSAFOL_Sort.
-
-(* Sorts of many-sorted algebra*)
-Inductive MSA_sorts : Set :=
+Inductive MSFOL_sorts : Set :=
 | Nat
 | List
 | Cfg
 | Term
 .
 
-(* a function which corresponds: constants of AML  to  sorts of MSA *)
-Fixpoint AML_sort_name (s : MSA_sorts) : Sigma_pattern :=
-match s with
-| Nat  => const ("Nat")
-| List => const ("List")
-| Cfg  => const ("Cfg")
-| Term => const ("Term")
+Inductive MSFOL_var : Type :=
+| M_var_c (id_M_var : string) (sort_M_var : MSFOL_sorts).
+Inductive MSFOL_fun : Type := M_fun_c {id_M_fun : string}.
+
+Definition msort_eq_dec : forall (x y : MSFOL_sorts), { x = y } + { x <> y }.
+Proof. decide equality. Defined.
+
+Definition mvar_eq_dec : forall (x y : MSFOL_var), { x = y } + { x <> y }.
+Proof.
+  decide equality.
+  exact (msort_eq_dec sort_M_var sort_M_var0).
+  exact (string_dec id_M_var id_M_var0).
+Defined.
+
+Inductive MSFOL_term : Type :=
+| MT_var (x_s : MSFOL_var)
+| MT_fun (f : MSFOL_fun) {n : nat} (params : VectorDef.t MSFOL_term n)
+         (result_sort : MSFOL_sorts)
+.
+
+Inductive MSFOL_pred : Type := M_pred_c {id_M_pred : string}.
+
+Inductive MSFOL_formula : Set :=
+| MF_pred (p : MSFOL_pred) {n : nat} (params : VectorDef.t MSFOL_term n)
+| MF_bottom
+| MF_impl (l r : MSFOL_formula)
+| MF_exists (x : MSFOL_var) (phi : MSFOL_formula)
+.
+
+Notation "'M_Bot'" := (MF_bottom).
+Notation "a 'M~>' b" := (MF_impl a b) (at level 90, right associativity,
+                                       b at level 200).
+Notation "'M_ex' x , phi" := (MF_exists x phi) (at level 55).
+
+(* Derived notations *)
+Definition MF_not (phi : MSFOL_formula) := phi M~> M_Bot.
+Notation "'M¬' phi" := (MF_not phi) (at level 75).
+
+Definition MF_or  (l r : MSFOL_formula) := (M¬ l) M~> r.
+Notation "a M|_ b" := (MF_or a b) (at level 85, right associativity).
+
+Definition MF_and (l r : MSFOL_formula) := M¬ ((M¬ l) M|_ (M¬ r)).
+Notation "a M&_ b" := (MF_and a b) (at level 80, right associativity).
+
+Definition MF_iff (l r : MSFOL_formula) := ((l M~> r) M&_ (l M~> r)).
+Notation "a <M~> b" := (MF_iff a b) (at level 95, no associativity).
+
+Definition MF_top := (M¬ MF_bottom).
+Notation "'M_Top'" := MF_top.
+
+Definition MF_forall (x : MSFOL_var) (phi : MSFOL_formula) :=
+  M¬ (MF_exists x (M¬ phi)).
+Notation "'M_all' x , phi" := (MF_forall x phi) (at level 55).
+
+(* auxiliaty functions for equality checking *)
+Definition MSFOL_sorts_eqb (a b : MSFOL_sorts) : bool :=
+match a, b with
+| Nat, Nat => true
+| List, List => true
+| Cfg, Cfg => true
+| Term, Term => true
+| _, _ => false
 end.
 
-Definition Domain_Symbol := const ("Domain symbol").
+(* Definition mvar_eq (x y : MSFOL_var) : bool :=
+match x, y with
+| (M_var_c id_x sort_x), (M_var_c id_y sort_y) =>
+    andb (String.eqb id_x id_y) (MSFOL_sorts_eqb sort_x sort_y)
+end. *)
 
-Definition Domain (sort : MSA_sorts) := Domain_Symbol $ (AML_sort_name sort).
+
+(* Substitue varibale in term *)
+Fixpoint t_subst_var (term : MSFOL_term) (t : MSFOL_term) (x : MSFOL_var)
+: MSFOL_term :=
+match term with
+| MT_var x' => if mvar_eq_dec x x' then t else (MT_var x')
+| MT_fun f params result_sort =>
+    MT_fun f (VectorDef.map (fun y => t_subst_var y t x) params) result_sort
+end.
+
+(* Substitue varibale in formula *)
+Fixpoint f_subst_var (phi : MSFOL_formula) (t : MSFOL_term) (x : MSFOL_var)
+: MSFOL_formula :=
+match phi with
+| MF_pred p params =>
+    MF_pred p (VectorDef.map (fun y => t_subst_var y t x) params)
+| MF_bottom => MF_bottom
+| MF_impl lhs rhs => MF_impl (f_subst_var lhs t x) (f_subst_var rhs t x)
+| MF_exists x' formula => if mvar_eq_dec x x'
+                          then M_ex x', formula
+                          else M_ex x', (f_subst_var formula t x)
+end.
+
+
+Definition M_set_singleton := fun x => set_add mvar_eq_dec x List.nil.
+
+Fixpoint var_to_set (term : MSFOL_term)
+: ListSet.set MSFOL_var -> ListSet.set MSFOL_var :=
+match term with
+| MT_var x' => set_add mvar_eq_dec x'
+| MT_fun f _ _ => set_union mvar_eq_dec (empty_set MSFOL_var)
+end.
+
+(* free variables of a formula *)
+Fixpoint f_free_vars (phi : MSFOL_formula) : (ListSet.set MSFOL_var) :=
+match phi with
+| MF_pred p params =>
+    VectorDef.fold_right var_to_set params (empty_set MSFOL_var)
+| MF_bottom => List.nil
+| MF_impl lhs rhs => set_union mvar_eq_dec (f_free_vars lhs) (f_free_vars rhs)
+| MF_exists y phi' => set_diff mvar_eq_dec (f_free_vars phi') (M_set_singleton y)
+end.
+
+
+(* record MSFOL_structure := {
+  Domain : SortType (* subset of SortSet *)
+  Function_interp : MSFOL_fun -> Domain* -> Domain -> value_type?
+  Predicate_interp : MSFOL_pred -> Domain* -> value_type?
+}. *)
+
+(* Fixpoint MSFOL_term_valuation (t : MSFOL_term) : MSFOL_sorts :=
+match t with
+| MT_var x => (* result will have type: match x with M_var_c name sort => sort end *)
+| MT_fun f params r_sort => (* result will have type: r_sort *)
+end.
+
+Fixpoint MSFOL_formula_valuation (formula : MSFOL_formula) : bool :=
+match formula with
+| MF_pred p params => ?
+| MF_bottom => false
+| MF_impl phi1 phi2 =>
+    not (MSFOL_formula_valuation phi1) /\ (MSFOL_formula_valuation phi2)
+| MP_exists x phi => ?
+. *)
+
+(* Deifinition satisfies_model (A : ?) (phi : MSFOL_formula) : Prop :=
+  forall valutaion : ?, valuation phi A = true. *)
+
+(* Definition satisfies_theory (A : ?) (Omega : Ensemle MSFOL_formula) : Prop :=
+  forall axiom : MSFOL_formula, In _ axiom A -> satisfies_model A axiom. *)
+
+(* Definition satisfies
+(Omega : Ensemble MSFOL_formula) (phi : MSFOL_formula) : Prop :=
+  forall A : ?, satisfies_theory A Omega -> stisfies_model A phi. *)
+
+(* Auxiliary axiom schemes for proving propositional tautology *)
+Reserved Notation "pattern 'MSFOL_tautology'" (at level 2).
+Inductive MSFOL_tautology_proof_rules : MSFOL_formula -> Prop :=
+| MSFOL_p1 (phi : MSFOL_formula) :
+    (phi M~> phi) MSFOL_tautology
+
+| MSFOL_p2 (phi psi : MSFOL_formula) :
+    (phi M~> (psi M~> phi)) MSFOL_tautology
+
+| MSFOL_p3 (phi psi xi : MSFOL_formula) :
+    ((phi M~> (psi M~> xi)) M~> ((phi M~> psi) M~> (phi M~> xi))) MSFOL_tautology
+
+| MSFOL_p4 (phi psi : MSFOL_formula) :
+    (((M¬ phi) M~> (M¬ psi)) M~> (psi M~> phi)) MSFOL_tautology
+
+where "pattern 'MSFOL_tautology'" := (MSFOL_tautology_proof_rules pattern).
+
+Reserved Notation "pattern 'MSFOL_proved'" (at level 2).
+Inductive MSFOL_proof_system : MSFOL_formula -> Prop :=
+(* Propositional tautology *)
+| MSFOL_prop_tau (phi : MSFOL_formula) :
+    phi MSFOL_tautology -> phi MSFOL_proved
+
+(* Modus ponens *)
+| MSFOL_mod_pon {phi1 phi2 : MSFOL_formula} :
+    phi1 MSFOL_proved -> (phi1 M~> phi2) MSFOL_proved -> phi2 MSFOL_proved
+
+(* Existential quantifier *)
+| MSFOL_ex_quan {phi : MSFOL_formula} {x : MSFOL_var} {t : MSFOL_term}:
+    ((f_subst_var phi t x) M~> (M_ex x, phi)) MSFOL_proved
+
+(* Existential generalization *)
+| MSFOL_ex_gen (phi1 phi2 : MSFOL_formula) (x : MSFOL_var) :
+    (phi1 M~> phi2) MSFOL_proved ->
+    negb (set_mem mvar_eq_dec x (f_free_vars phi2)) = true ->
+    ((M_ex x, phi1) M~> phi2) MSFOL_proved
+
+where "phi 'MSFOL_proved'" := (MSFOL_proof_system phi).
+
+
+(* Section 4.2 *)
+Definition MSAFOL_Sort := const ("Sort").
+
+(* a function which corresponds: constants of AML  to  sorts of MSFOL *)
+Fixpoint sort_fun_constant (s : MSFOL_sorts) : Sigma_pattern :=
+match s with
+| Nat  => Functional_Constant (sigma_c("Nat"))
+| List => Functional_Constant (sigma_c("List"))
+| Cfg  => Functional_Constant (sigma_c("Cfg"))
+| Term => Functional_Constant (sigma_c("Term"))
+end.
+
+Fixpoint sort_constant (s : MSFOL_sorts) : Sigma :=
+match s with
+| Nat  => (sigma_c("Nat"))
+| List => (sigma_c("List"))
+| Cfg  => (sigma_c("Cfg"))
+| Term => (sigma_c("Term"))
+end.
+
+Definition Axiom_Sort (s : MSFOL_sorts) := (sort_constant s) -< MSAFOL_Sort.
+
+
+Definition Domain_Symbol := const ("Domain symbol").
+Definition Domain (sort : MSFOL_sorts) := Domain_Symbol $ ^(sort_constant sort).
 Notation "'[[' s ']]'" := (Domain s) (at level 0).
 
-Definition Nonempty_Domain (sort : MSA_sorts) :=  [[ sort ]] !=~ sp_bottom.
+(* Examples meanings: *)
+(* x =< [[ s ]] states that x has sort s *)
+Definition x_has_sort_s (x : EVar) (s : MSFOL_sorts) :=
+  x =< [[ s ]].
 
-(* Instead of notation "forall x : Nat . pattern" we introduce: *)
-Notation "'ex_M' x : sort , phi" :=
-  (sp_exists x ((Membership x ([[ sort ]])) _&_ phi)) (at level 3, x at next level, sort at next level).
-Notation "'all_M' x : sort , phi" :=
-  (sp_forall x ((Membership x ([[ sort ]])) ~> phi)) (at level 3, x at next level, sort at next level).
+(* phi <: [[ s ]] states that all elements matching phi have sort s*)
+Definition pattern_has_sort (phi : Sigma_pattern) (s : MSFOL_sorts) :=
+  phi <: [[ s ]].
 
+Definition Nonempty_Domain (sort : MSFOL_sorts) :=  [[ sort ]] !=~ sp_bottom.
 
-Reserved Notation "a |--> b" (at level 40, left associativity).
-Inductive QuantificationEquivalence : Sigma_pattern -> Sigma_pattern -> Prop :=
-| QE_ex_to_all (x : EVar) (s : MSA_sorts) (phi : Sigma_pattern) :
-    ((ex_M x : s, phi) |--> (¬ (all_M x : s, (¬ phi))))
-| QE_all_to_ex (x : EVar) (s : MSA_sorts) (phi : Sigma_pattern) :
-    ((all_M x : s, phi)  |--> (¬ (ex_M x : s, (¬ phi))))
-where "a |--> b" := (QuantificationEquivalence a b).
+(* Introducing notations for Sorted quantification *)
+(* For denoting "exists x : Nat . pattern" we introduce: *)
+Notation "'ex_S' x : sort , phi" :=
+  (sp_exists x ((x =< ([[ sort ]])) _&_ phi)) (at level 3, x at next level, sort at next level).
+(* For denoting "forall x : Nat . pattern" we introduce: *)
+Notation "'all_S' x : sort , phi" :=
+  (sp_forall x ((x =< ([[ sort ]])) ~> phi)) (at level 3, x at next level, sort at next level).
+
 
 (* Proposition 10. *)
-(* Lemma forall_ex_equiv :
-  forall s : MSA_sorts, forall x : EVar, forall phi : Sigma_pattern,
-  (Empty_set _) |-
-    (all_M x : sort, phi) ~=~ (¬ (ex_M x : sort, (¬ phi))). *)
+Reserved Notation "a |--> b" (at level 40, left associativity).
+Inductive QuantificationEquivalence : Sigma_pattern -> Sigma_pattern -> Prop :=
+| QE_ex_to_all (x : EVar) (s : MSFOL_sorts) (phi : Sigma_pattern) :
+    ((ex_S x : s, phi) |--> (¬ (all_S x : s, (¬ phi))))
+| QE_all_to_ex (x : EVar) (s : MSFOL_sorts) (phi : Sigma_pattern) :
+    ((all_S x : s, phi)  |--> (¬ (ex_S x : s, (¬ phi))))
+where "a |--> b" := (QuantificationEquivalence a b).
 
+Lemma forall_ex_equiv :
+  forall s : MSFOL_sorts, forall x : EVar, forall phi : Sigma_pattern,
+  empty_theory |- ((all_S x:s, phi) ~=~ (¬ (ex_S x:s, (¬ phi)))).
+Admitted.
+
+
+(* Many-sorted functions and terms *)
 Section NatToStringConversion.
 
 Local Open Scope string_scope.
@@ -904,20 +1113,18 @@ end.
 Fixpoint gen_x_vec (n : nat) : VectorDef.t EVar n :=
   _gen_x_vec n n.
 
-(* TODO: FunctionBase : \/x:s.\/y:t ... . phi *)
-Definition y := evar_c("y").
 Fixpoint Function
-  {n : nat} (fn : Sigma) (sorts : VectorDef.t MSA_sorts n) (sy : MSA_sorts)
+  {n : nat} (fn : Sigma) (sorts : VectorDef.t MSFOL_sorts n) 
+  (y_sort : MSFOL_sorts)
 : Sigma_pattern :=
 let vars := gen_x_vec n in
-let var_pats := VectorDef.map sp_var vars in
-let applied_params := VectorDef.fold_left sp_app (sp_const fn) var_pats in
-let core := ex_M y : sy, applied_params in
+let var_patterns := VectorDef.map sp_var vars in
+let applied_params := VectorDef.fold_left sp_app (sp_const fn) var_patterns in
+let core := ex_S (evar_c("y")) : y_sort, (applied_params ~=~ (var ("y")) )in
 let foralls := VectorDef.map2
-                (fun var s => (fun phi => all_M var : s, phi))
+                (fun var s => (fun phi => all_S var : s, phi))
                 vars sorts in
   VectorDef.fold_right (fun spl spr => spl spr) foralls core.
-
 
 (* Functional notation of the function *)
 Notation "f : '-->' s" := (Function f (vn _) s) (at level 3).
@@ -925,33 +1132,53 @@ Notation "f : s1 '-->' s" := (Function f (vc _ s1 0 (vn _)) s) (at level 3).
 Notation "f : s1 'X' s2 'X' .. 'X' sn '-->' s" :=
   (Function f (vc _ s1 _ (vc _ s2 _ .. (vc _ sn _ (vn _)) .. )) s) (at level 3).
 
-(* Examples for functional notation *)
-Definition zero : Sigma := sigma_c("zero").
-Definition succ : Sigma := sigma_c("succ").
-Definition plus : Sigma := sigma_c("plus'").
-Definition mult : Sigma := sigma_c("mult").
-
-Definition zero_fun := (zero : --> Nat).
-Definition succ_fun := (succ : Nat --> Nat).
-Definition plus_fun := (plus : Nat X Nat --> Nat).
-Definition mult_fun := (mult : Nat X Nat --> Nat).
+(* Example for functional notation *)
+Definition f := (sigma_c "f") : --> List.
+Definition fib := (sigma_c "fib") : Nat --> Nat.
+Definition volume := (sigma_c "volume") : Nat X Nat --> Nat.
 
 
+(* Many-sorted predicates and formulas *)
 Definition Predicate
-  {n : nat} (fn : Sigma) (sorts : VectorDef.t MSA_sorts n)
+  {n : nat} (fn : Sigma) (sorts : VectorDef.t MSFOL_sorts n)
 : Sigma_pattern :=
 let vars := gen_x_vec n in
-let var_pats := VectorDef.map sp_var vars in
-let applied_params := VectorDef.fold_left sp_app (sp_const fn) var_pats in
+let var_patterns := VectorDef.map sp_var vars in
+let applied_params := VectorDef.fold_left sp_app (sp_const fn) var_patterns in
 let or_left := applied_params ~=~ Top in
 let or_right := applied_params ~=~ Bot in
 let core := or_left _|_ or_right in
 let foralls := VectorDef.map2
-                (fun var s => (fun phi => (all_M var : s, phi)))
+                (fun var s => (fun phi => (all_S var : s, phi)))
                 vars sorts in
   VectorDef.fold_right (fun spl spr => spl spr) foralls core.
 
-Fixpoint and_gen {n : nat} (vec : VectorDef.t Sigma_pattern n)
+
+(* well-sorted axiom scheme *)
+Fixpoint get_vars (term : MSFOL_term) : Sigma_pattern -> Sigma_pattern :=
+match term with
+| MT_var x => match x with
+    M_var_c id sort => sp_and ((evar_c(id)) =< [[ sort ]]) end
+| MT_fun f params r_sort => VectorDef.fold_right get_vars params
+end.
+
+Fixpoint well_sorted_term (term : MSFOL_term) : Sigma_pattern :=
+match term with
+| MT_var x => match x with M_var_c id sort => ((evar_c(id)) =< [[ sort ]]) end
+| MT_fun f params r_sort => VectorDef.fold_right get_vars params Top
+end.
+
+Fixpoint well_sorted_formula (formula : MSFOL_formula) : Sigma_pattern :=
+match formula with
+| MF_pred p params => VectorDef.fold_right get_vars params Top
+| MF_bottom => Top
+| MF_impl lhs rhs => sp_and (well_sorted_formula lhs) (well_sorted_formula rhs)
+| MF_exists x phi =>
+    sp_and (match x with M_var_c id sort => ((evar_c(id)) =< [[ sort ]]) end)
+           (well_sorted_formula phi)
+end.
+
+(* Fixpoint and_gen {n : nat} (vec : VectorDef.t Sigma_pattern n)
 : Sigma_pattern :=
 match vec with
 | VectorDef.nil  _                          => sp_top (* TODO: sp_top? *)
@@ -964,7 +1191,7 @@ Definition _well_sorted
 : Sigma_pattern :=
 let domains := VectorDef.map Domain sorts in
 let assoc := VectorDef.map2 Membership vars domains in
-  and_gen assoc.
+  and_gen assoc. *)
 
 (* TODO: fix this and ask how to get types?
         Answer: from MSFOL format of variables, because they have the form of x:s
@@ -976,23 +1203,102 @@ let vars := of_list (free_vars phi) in
 
 (* TODO: MSFOL theory conversion to AML conversion *)
 
+
 (* Proposition 12. *)
-(* Theorem MSFOL_wellformed : forall phi : Sigma_pattern,
-  Gamma_MSFOL |- (ws phi) ~> ((phi ~=~ sp_top) _|_ (phi ~=~ sp_bottom)). *)
+Fixpoint M_var_id (var : MSFOL_var) : string :=
+match var with M_var_c id _ => id end.
+
+Fixpoint M_var_sort (var : MSFOL_var) : MSFOL_sorts :=
+match var with M_var_c _ sort => sort end.
+
+Fixpoint term_sort (term : MSFOL_term) : MSFOL_sorts :=
+match term with
+| MT_var x => match x with M_var_c _ sort => sort end
+| MT_fun _ _ result_sort => result_sort
+end.
+
+Fixpoint term_to_AML (term : MSFOL_term) : Sigma_pattern:=
+match term with
+| MT_var x => match x with M_var_c id _ => var id end
+| MT_fun f_id params result_sort =>
+    match f_id with (M_fun_c id) =>
+      Function (sigma_c id)
+               (VectorDef.map term_sort params)
+               result_sort
+    end
+end.
+
+Fixpoint formula_to_AML (formula : MSFOL_formula) : Sigma_pattern :=
+match formula with
+| MF_pred p params => 
+    match p with M_pred_c id =>
+      Predicate (sigma_c id) (VectorDef.map term_sort params)
+    end
+| MF_bottom => Bot
+| MF_impl lhs rhs => (formula_to_AML lhs) ~> (formula_to_AML rhs)
+| MF_exists x phi =>
+    ex_S (evar_c (M_var_id x)) : (M_var_sort x) , (formula_to_AML phi)
+end.
+
+
+Lemma MSFOL_wellformed_terms :
+  forall Gamma_MSFOL : Ensemble Sigma_pattern, forall t : MSFOL_term,
+  Gamma_MSFOL |- ((well_sorted_term t) ~>
+    ex_S (evar_c("y")) : (term_sort t), (term_to_AML t) ~=~ (var "y")).
+Admitted.
+
+Lemma MSFOL_wellformed_formulas :
+  forall Gamma_MSFOL : Ensemble Sigma_pattern, forall phi : MSFOL_formula,
+  Gamma_MSFOL |- ((well_sorted_formula phi) ~>
+    ((formula_to_AML phi) ~=~ sp_top) _|_ (((formula_to_AML phi) ~=~ sp_bottom))).
+Admitted.
+
+(* MSFOL theories *)
 
 (* Theorem 13. *)
-(* Theorem Omega |- MSFOL phi -> Gamma_MSFOL |- phiMSFOL. *)
+(* Theorem preservation :
+  forall Omega : Ensemble MSFOL_formula, forall Gamma : Ensemble Sigma_pattern,
+  forall phi : MSFOL_formula
+  Omega |-MSFOL phi -> Gamma_MSFOL |- (formula_to_AML phi). *)
 
 (* Definition 14. MSFOL restricted *)
 
+
 (* Theorem 15. *)
+(* Theorem 
+  forall Omega : Ensemble MSFOL_formula, forall A : MSFOL_model,
+  A |=MSFOL Omega -> exists M : Sigma_model, ... *)
 
 (* Theorem 16. *)
+(* Theorem holds :
+  forall Omega : Ensemble MSFOL_formula, phi : MSFOL_formula,
+  let Gamma := (theory_to_AML Omega) in
+    (Omega |-MSFOL phi -> Gamma |- (formula_to_AML phi)) /\
+    (Gamma |- (formula_to_AML phi) -> Gamma |= (formula_to_AML phi)) /\
+    (Gamma |= (formula_to_AML phi) -> Omega |=MSFOL phi) /\
+    (Omega |=MSFOL phi -> Omega |-MSFOL phi).
+ *)
 
-(* Natural numbers *)
+
+(* ************************************************************************** *)
+(*                           ~= Natural numbers =~                            *)
+(* ************************************************************************** *)
+
+Definition zero : Sigma := sigma_c("zero").
+Definition succ : Sigma := sigma_c("succ").
+Definition plus : Sigma := sigma_c("plus'").
+Definition mult : Sigma := sigma_c("mult").
+
+Definition zero_fun := (zero : --> Nat).
+Definition succ_fun := (succ : Nat --> Nat).
+Definition plus_fun := (plus : Nat X Nat --> Nat).
+Definition mult_fun := (mult : Nat X Nat --> Nat).
+
+(* Helper functions for notation *)
 Definition succ' (x : Sigma_pattern) := ^succ $ x.
 Definition plus' (x y : Sigma_pattern) := ^plus $ x $ y.
 Definition mult' (x y : Sigma_pattern) := ^mult $ x $ y.
+(* End helper functions *)
 
 Definition No_Confusion1 (x : EVar) :=
   all_M x : Nat, ((succ' 'x) !=~ (const ("zero"))).
